Changes designed to simplify boolifying variables.

src/Boolify/src/CoderScript.sml
@@ -28,14 +28,6 @@ val Know = Q_TAC KNOW_TAC;
 val REVERSE = Tactical.REVERSE;
 
 (*---------------------------------------------------------------------------
-     Well-formed encoder/decoder pairs.
- ---------------------------------------------------------------------------*)
-
-val wf_coder_def =
- Define
- `wf_coder p (e : 'a -> bool list) d = wf_encoder p e /\ (d = enc2dec p e)`;
-
-(*---------------------------------------------------------------------------
      decode turns a decoding parser of type
 
        bool list -> ('a # bool list) option
@@ -45,7 +37,34 @@ val wf_coder_def =
        bool list -> 'a
  ---------------------------------------------------------------------------*)
 
-val decode_def = Define `decode f x = FST (THE (f x))`;
+val decode_def =
+  Define
+  `decode (p : 'a -> bool) (d : bool list -> ('a # bool list) option) l =
+   case d l of SOME (x, _) -> x || NONE -> @x. p x`;
+
+(*---------------------------------------------------------------------------
+     Well-formed (predicate,encoder,decoder) triples.
+ ---------------------------------------------------------------------------*)
+
+val wf_coder_def =
+  Define
+  `wf_coder (p, e, d) = wf_pred p /\ wf_encoder p e /\ (d = enc2dec p e)`;
+
+val domain_def =
+  Define
+  `domain
+   (p : 'a->bool, e : 'a->bool list, d : bool list->('a#bool list) option) = p`;
+
+val encoder_def =
+  Define
+  `encoder
+   (p : 'a->bool, e : 'a->bool list, d : bool list->('a#bool list) option) = e`;
+
+val decoder_def =
+  Define
+  `decoder
+   (p : 'a->bool, e : 'a->bool list, d : bool list->('a#bool list) option) =
+   decode p d`;
 
 (*---------------------------------------------------------------------------
      Well-formed coders have nice properties for boolification.
@@ -53,7 +72,7 @@ val decode_def = Define `decode f x = FST (THE (f x))`;
 
 val decode_encode = store_thm
   ("decode_encode",
-   ``!p e x. wf_encoder p e /\ p x ==> (decode (enc2dec p e) (e x) = x)``,
+   ``!p e x. wf_encoder p e /\ p x ==> (decode p (enc2dec p e) (e x) = x)``,
    RW_TAC std_ss [] ++
    Cases_on `enc2dec p e (e x)` >>
    (POP_ASSUM MP_TAC ++
@@ -70,17 +89,33 @@ val decode_encode = store_thm
 
 val wf_coder = store_thm
   ("wf_coder",
-   ``!p e d.
-       wf_coder p (e : 'a -> bool list) d ==>
-       !x. p x ==> (decode d (e x) = x)``,
-   RW_TAC std_ss [wf_coder_def, decode_encode]);
+   ``!c.
+       wf_coder c ==>
+       !x. domain c x ==> (decoder c (encoder c x) = x)``,
+   Cases
+   ++ Cases_on `r`
+   ++ RW_TAC std_ss
+      [wf_coder_def, decode_encode, encoder_def, decoder_def, domain_def]);
+
+val wf_coder_closed = store_thm
+  ("wf_coder_closed",
+   ``!c. wf_coder c ==> !l. domain c (decoder c l)``,
+   Cases
+   ++ Cases_on `r`
+   ++ RW_TAC std_ss
+      [wf_coder_def, domain_def, decoder_def, decode_def, wf_pred_def]
+   ++ REPEAT CASE_TAC >> (HO_MATCH_MP_TAC SELECT_AX ++ PROVE_TAC [])
+   ++ POP_ASSUM MP_TAC
+   ++ RW_TAC std_ss [enc2dec_some]);
 
 val wf_coder_op = store_thm
   ("wf_coder_op",
    ``!p e f.
-       wf_encoder p e /\ (!x. p x ==> (e x = f x)) ==>
-       wf_coder p e (enc2dec p f)``,
-   RW_TAC std_ss [wf_coder_def]
+       (?x. p x) /\ wf_encoder p e /\ (!x. p x ==> (e x = f x)) ==>
+       wf_coder (p, e, enc2dec p f)``,
+   RW_TAC std_ss [wf_coder_def, wf_pred_def]
+   ++ Q.UNDISCH_TAC `p x`
+   ++ DISCH_THEN (K ALL_TAC)
    ++ MATCH_MP_TAC EQ_EXT
    ++ RW_TAC std_ss []
    ++ Know `wf_encoder p f` >> HO_METIS_TAC [wf_encoder_eq]
@@ -104,8 +139,10 @@ val wf_coder_op = store_thm
 
 val wf_coder_unit = store_thm
   ("wf_coder_unit",
-   ``!p. wf_coder p encode_unit (decode_unit p)``,
-   RW_TAC std_ss [wf_encode_unit, decode_unit_def, wf_coder_def]);
+   ``!p. p () ==> wf_coder (p, encode_unit, decode_unit p)``,
+   RW_TAC std_ss [wf_encode_unit, decode_unit_def, wf_coder_def, wf_pred_def]
+   ++ Q.EXISTS_TAC `()`
+   ++ RW_TAC std_ss []);
 
 (*---------------------------------------------------------------------------
      Boolean coders
@@ -113,7 +150,7 @@ val wf_coder_unit = store_thm
 
 val wf_coder_bool = store_thm
   ("wf_coder_bool",
-   ``!p. wf_coder p encode_bool (decode_bool p)``,
+   ``!p. wf_pred p ==> wf_coder (p, encode_bool, decode_bool p)``,
    RW_TAC std_ss [wf_encode_bool, decode_bool_def, wf_coder_def]);
 
 (*---------------------------------------------------------------------------
@@ -123,12 +160,13 @@ val wf_coder_bool = store_thm
 val wf_coder_prod = store_thm
   ("wf_coder_prod",
    ``!p1 p2 (e1 : 'a -> bool list) (e2 : 'b -> bool list) d1 d2.
-       wf_coder p1 e1 d1 /\ wf_coder p2 e2 d2 ==>
-       wf_coder (lift_prod p1 p2) (encode_prod e1 e2)
-       (decode_prod (lift_prod p1 p2) d1 d2)``,
+       wf_coder (p1, e1, d1) /\ wf_coder (p2, e2, d2) ==>
+       wf_coder (lift_prod p1 p2, encode_prod e1 e2,
+                 decode_prod (lift_prod p1 p2) d1 d2)``,
    RW_TAC std_ss [decode_prod_def]
    ++ MATCH_MP_TAC wf_coder_op
-   ++ FULL_SIMP_TAC std_ss [wf_coder_def, wf_encode_prod]
+   ++ FULL_SIMP_TAC std_ss [wf_coder_def, wf_encode_prod, wf_pred_def]
+   ++ CONJ_TAC >> (Q.EXISTS_TAC `(x, x')` ++ RW_TAC std_ss [lift_prod_def])
    ++ Cases
    ++ RW_TAC std_ss [encode_prod_def, lift_prod_def, dec2enc_enc2dec]);
 
@@ -139,12 +177,13 @@ val wf_coder_prod = store_thm
 val wf_coder_sum = store_thm
   ("wf_coder_sum",
    ``!p1 p2 (e1 : 'a -> bool list) (e2 : 'b -> bool list) d1 d2.
-       wf_coder p1 e1 d1 /\ wf_coder p2 e2 d2 ==>
-       wf_coder (lift_sum p1 p2) (encode_sum e1 e2)
-       (decode_sum (lift_sum p1 p2) d1 d2)``,
+       wf_coder (p1, e1, d1) /\ wf_coder (p2, e2, d2) ==>
+       wf_coder (lift_sum p1 p2, encode_sum e1 e2,
+                 decode_sum (lift_sum p1 p2) d1 d2)``,
    RW_TAC std_ss [decode_sum_def]
    ++ MATCH_MP_TAC wf_coder_op
-   ++ FULL_SIMP_TAC std_ss [wf_coder_def, wf_encode_sum]
+   ++ FULL_SIMP_TAC std_ss [wf_coder_def, wf_encode_sum, wf_pred_def]
+   ++ CONJ_TAC >> (Q.EXISTS_TAC `INL x` ++ RW_TAC std_ss [lift_sum_def])
    ++ Cases
    ++ RW_TAC std_ss [encode_sum_def, lift_sum_def, dec2enc_enc2dec]);
 
@@ -155,12 +194,13 @@ val wf_coder_sum = store_thm
 val wf_coder_option = store_thm
   ("wf_coder_option",
    ``!p (e : 'a -> bool list) d.
-       wf_coder p e d ==>
-       wf_coder (lift_option p) (encode_option e)
-       (decode_option (lift_option p) d)``,
+       wf_coder (p, e, d) ==>
+       wf_coder (lift_option p, encode_option e,
+                 decode_option (lift_option p) d)``,
    RW_TAC std_ss [decode_option_def]
    ++ MATCH_MP_TAC wf_coder_op
-   ++ FULL_SIMP_TAC std_ss [wf_coder_def, wf_encode_option]
+   ++ FULL_SIMP_TAC std_ss [wf_coder_def, wf_encode_option, wf_pred_def]
+   ++ CONJ_TAC >> (Q.EXISTS_TAC `NONE` ++ RW_TAC std_ss [lift_option_def])
    ++ Induct
    ++ RW_TAC std_ss [encode_option_def, lift_option_def, dec2enc_enc2dec]);
 
@@ -171,11 +211,12 @@ val wf_coder_option = store_thm
 val wf_coder_list = store_thm
   ("wf_coder_list",
    ``!p (e : 'a -> bool list) d.
-       wf_coder p e d ==>
-       wf_coder (EVERY p) (encode_list e) (decode_list (EVERY p) d)``,
+       wf_coder (p, e, d) ==>
+       wf_coder (EVERY p, encode_list e, decode_list (EVERY p) d)``,
    RW_TAC std_ss [decode_list_def]
    ++ MATCH_MP_TAC wf_coder_op
-   ++ FULL_SIMP_TAC std_ss [wf_coder_def, wf_encode_list]
+   ++ FULL_SIMP_TAC std_ss [wf_coder_def, wf_encode_list, wf_pred_def]
+   ++ CONJ_TAC >> (Q.EXISTS_TAC `[]` ++ RW_TAC std_ss [EVERY_DEF])
    ++ Induct
    ++ RW_TAC std_ss [encode_list_def, EVERY_DEF, dec2enc_enc2dec]);
 
@@ -185,7 +226,7 @@ val wf_coder_list = store_thm
 
 val wf_coder_num = store_thm
   ("wf_coder_num",
-   ``!p. wf_coder p encode_num (decode_num p)``,
+   ``!p. wf_pred p ==> wf_coder (p, encode_num, decode_num p)``,
    RW_TAC std_ss [wf_encode_num, decode_num_def, wf_coder_def]);
 
 (*---------------------------------------------------------------------------
@@ -194,8 +235,10 @@ val wf_coder_num = store_thm
 
 val wf_coder_bnum = store_thm
   ("wf_coder_bnum",
-   ``!m p. wf_pred_bnum m p ==> wf_coder p (encode_bnum m) (decode_bnum m p)``,
-   RW_TAC std_ss [wf_encode_bnum, decode_bnum_def, wf_coder_def]);
+   ``!m p. wf_pred_bnum m p ==> wf_coder (p, encode_bnum m, decode_bnum m p)``,
+   RW_TAC std_ss [wf_encode_bnum, decode_bnum_def, wf_coder_def]
+   ++ FULL_SIMP_TAC std_ss [wf_pred_bnum_def]
+   ++ PROVE_TAC []);
 
 (*---------------------------------------------------------------------------
      Tree coders
@@ -204,11 +247,13 @@ val wf_coder_bnum = store_thm
 val wf_coder_tree = store_thm
   ("wf_coder_tree",
    ``!p (e : 'a -> bool list) d.
-       wf_coder p e d ==>
-       wf_coder (lift_tree p) (encode_tree e) (decode_tree (lift_tree p) d)``,
+       wf_coder (p, e, d) ==>
+       wf_coder (lift_tree p, encode_tree e, decode_tree (lift_tree p) d)``,
    RW_TAC std_ss [decode_tree_def]
    ++ MATCH_MP_TAC wf_coder_op
-   ++ FULL_SIMP_TAC std_ss [wf_coder_def, wf_encode_tree]
+   ++ FULL_SIMP_TAC std_ss [wf_coder_def, wf_encode_tree, wf_pred_def]
+   ++ CONJ_TAC
+   >> (Q.EXISTS_TAC `Node x []` ++ RW_TAC std_ss [lift_tree_def, EVERY_DEF])
    ++ HO_MATCH_MP_TAC tree_ind
    ++ RW_TAC std_ss [encode_tree_def, lift_tree_def, dec2enc_enc2dec, APPEND_11]
    ++ Induct_on `ts`
